tactics: some arith work

ulib/FStar.Reflection.Arith.fst
@@ -37,21 +37,12 @@ let gt e1 e2 = CompProp e1 C_Gt e2
 let ge e1 e2 = CompProp (Plus (Lit 1) e1) C_Gt e2
 
 (* Define a traversal monad! Makes exception handling and counter-keeping easy *)
-private let tm a = nat -> option (a * nat)
-private let return (x:'a) : tm 'a = fun i -> Some (x, i)
+private let tm a = nat -> either string (a * nat)
+private let return (x:'a) : tm 'a = fun i -> Inr (x, i)
 private let bind (m : tm 'a) (f : 'a -> tm 'b) : tm 'b =
     fun i -> match m i with
-             | Some (x, j) -> f x j
-             | None -> None
-
-private let atom : tm nat = fun i -> Some (i, i + 1)
-private val fail : (#a:Type) -> tm a
-private let fail #a = fun i -> None
-
-let rec forall_list (p:'a -> Type) (l:list 'a) : Type =
-    match l with
-    | [] -> True
-    | x::xs -> p x /\ forall_list p xs
+             | Inl s -> Inl s
+             | Inr (x, j) -> f x j
 
 val liftM : ('a -> 'b) -> (tm 'a -> tm 'b)
 let liftM f x =
@@ -63,6 +54,17 @@ let liftM2 f x y =
     xx <-- x;
     yy <-- y;
     return (f xx yy)
+
+
+private let tick : tm nat = fun i -> Inr (i, i + 1)
+private let atom : tm expr = liftM Atom tick
+private val fail : (#a:Type) -> string -> tm a
+private let fail #a s = fun i -> Inl s
+
+let rec forall_list (p:'a -> Type) (l:list 'a) : Type =
+    match l with
+    | [] -> True
+    | x::xs -> p x /\ forall_list p xs
 
 let minus x y = Plus x (Neg y)
 
@@ -80,17 +82,21 @@ let rec is_arith_expr (t:term) =
         if      eq_qn qn add_qn   then liftM2 Plus ll rr
         else if eq_qn qn minus_qn then liftM2 minus ll rr
         else if eq_qn qn mult_qn  then liftM2 Mult ll rr
-        else fail
+        else fail "binary"
     | Tv_FVar fv, [a] ->
         let qn = inspect_fv fv in
         collect_app_order t;
         let aa = is_arith_expr (a <: x:term{x << t}) in
         if   eq_qn qn neg_qn then liftM Neg aa
-        else fail
+        else fail "unary"
     | Tv_Const (C_Int i), _ ->
         return (Lit i)
+    | Tv_FVar f , [] ->
+        atom
+    | Tv_Var f , [] ->
+        atom
     | _, _ ->
-        fail
+        fail "unk"
 
 val is_arith_prop : term -> tm prop
 let rec is_arith_prop (t:term) =
@@ -98,13 +104,13 @@ let rec is_arith_prop (t:term) =
     | Eq _ l r -> liftM2 eq (is_arith_expr l) (is_arith_expr r)
     | And l r  -> liftM2 AndProp (is_arith_prop l) (is_arith_prop r)
     | Or l r   -> liftM2  OrProp (is_arith_prop l) (is_arith_prop r)
-    | _ -> fail
+    | _ -> fail "connector"
 
 let test =
     let bind = FStar.Tactics.bind in
     let fail = FStar.Tactics.fail in
     assert_by_tactic (t <-- quote (1 + 2);
                              match is_arith_expr t 0 with
-                             | Some (Plus (Lit 1) (Lit 2), _) -> print "alright!"
-                             | _ -> fail "oops")
+                             | Inr (Plus (Lit 1) (Lit 2), _) -> print "alright!"
+                             | Inl s -> fail ("oops: " ^ s))
                             True
