examples/tactics/Arith.fst
@@ -11,16 +11,16 @@ let is_arith_goal : tactic bool =
     eg <-- cur_goal;
     let _, g = eg in
     match is_arith_prop g 0 with
-    | Some _ -> return true
-    | None -> return false
-
+    | Inr _ -> return true
+    | Inl s -> (print ("arith: not an arith prop: " ^ term_to_string g);;
+                print ("message: " ^ s);;
+                return false)
 
 val split_arith : unit -> Tac unit
 let rec split_arith = fun () -> (
-    addns ["Blah"];;
-    prune [];;
     b <-- is_arith_goal;
     if b then (
+        prune [];;
         addns ["Prims"];;
         smt
     ) else (
@@ -28,25 +28,39 @@ let rec split_arith = fun () -> (
         let _, g = eg in
         match term_as_formula g with
         | True_ -> trivial
-        //| And l r -> seq FStar.Tactics.split split_arith
+        | And l r -> seq FStar.Tactics.split split_arith
         | _ -> return ()
     )) ()
     
 
 // TODO: even if encoding this module to SMT, x is not given a HasType
-assume val x : int
+//assume val x : int
 
-let _ = assert_by_tactic (prune [];;
-                          FStar.Tactics.split;;
-                          (* rev part *)
-                            addns ["FStar";"List"];;
-                            addns ["Prims"];;
-                            smt;;
-                          (* arithmetic part *)
-                            addns ["Prims"];;
-                            addns ["Arith"];;
-                            smt;;
-                          return ()
-                         )
-                         (FStar.List.Tot.rev [1;2;3;4] == [4;3;2;1]
-                            /\ op_Multiply 2 (x + 3) == 6 + (op_Multiply 3 x) - x)
+let lem0 (x:int) =
+    assert_by_tactic (prune [];;
+                      addns ["Prims"]
+                     ) (op_Multiply 2 (x + 3) == 6 + (op_Multiply 3 x) - x)
+
+// Can't locally define tactics
+let tau1 : tactic unit =
+    prune [];;
+    FStar.Tactics.split;;
+    (* rev part *)
+      addns ["FStar";"List"];;
+      addns ["Prims"];;
+      smt;;
+    (* arithmetic part *)
+      addns ["Prims"];;
+      g <-- cur_goal;
+      let _, t = g in
+      print ("goal = " ^ term_to_string t);;
+      smt;;
+    return ()
+
+let lem1 (x:int) =
+    assert_by_tactic tau1 (FStar.List.Tot.rev [1;2;3;4] == [4;3;2;1]
+                             /\ op_Multiply 2 (x + 3) == 6 + (op_Multiply 3 x) - x)
+
+let lem2 (x:int) =
+    assert_by_tactic split_arith (FStar.List.Tot.rev [1;4] == [4;1]
+                                    /\ op_Multiply 2 (x + 3) == 6 + (op_Multiply 3 x) - x)
